thys/examples/sorting/IICF_Shared_Lists.thy
@@ -2,9 +2,6 @@ theory IICF_Shared_Lists
 imports "Isabelle_LLVM.IICF"
 begin
 
-section \<open>Lists with Element-wise Ownership\<close>
-
-
 (* TODO: Move *)  
 lemma list_all2_append2: "length xs' = length ys' \<Longrightarrow> list_all2 P (xs@xs') (ys@ys') \<longleftrightarrow> list_all2 P xs ys \<and> list_all2 P xs' ys'"  
   by (auto simp: list_all2_append list_all2_iff)
@@ -29,13 +26,25 @@ lemma map2_map_conv: "map2 f (map g xs) (map h ys) = map2 (\<lambda>x y. f (g x)
 lemma map2_same[simp]: "map2 f xs xs = map (\<lambda>x. f x x) xs"
   apply (induction xs) by auto
   
-  
-thm list.rel_map
+
+lemma nth_map2: "\<lbrakk> i<length xs; i<length ys \<rbrakk> \<Longrightarrow> map2 f xs ys ! i = f (xs!i) (ys!i)" by simp
+
+lemma map2_update1: "map2 f (xs[i:=x]) ys = (map2 f xs ys)[i := f x (ys!i)]"
+  by (metis list_update_id map_update old.prod.case zip_update)
+
+lemma map2_update2: "map2 f xs (ys[i:=y]) = (map2 f xs ys)[i := f (xs!i) y]"
+  by (metis list_update_id map_update old.prod.case zip_update)
+    
 lemma list_all2_map_map_conv: "list_all2 P (map f xs) (map g ys) = list_all2 (\<lambda>x y. P (f x) (g y)) xs ys"
   by (auto simp: list.rel_map)
   
-  
 
+
+section \<open>Lists with Element-wise Ownership\<close>
+
+
+  
+subsection \<open>Abstract Operations\<close>
 (* Split *)
 definition "sl_split s xs = map (\<lambda>i. if i\<in>s \<and> i<length xs then xs!i else None) [0..<length xs]"
 
@@ -69,11 +78,46 @@ definition "sl_get xs i = (if i<length xs then the (xs!i) else undefined (i-leng
 definition "sl_put xs i x = xs[i:=Some x]"
 
 
+subsection \<open>Lemmas for Abstract Operations\<close>
+
 lemma sl_indexes_alt: "sl_indexes' xs = {i . i<length xs \<and> xs!i \<noteq> None}"
   unfolding sl_indexes_def sl_struct_def
   by auto
 
+lemma sl_of_list_empty[simp]: "sl_of_list [] = []"
+  by (auto simp: sl_of_list_def)
 
+lemma sl_of_list_eq_empty_conv[simp]: "sl_of_list xs = [] \<longleftrightarrow> xs=[]"
+  by (auto simp: sl_of_list_def)
+
+lemma sl_split_empty[simp]: "sl_split s [] = []" by (auto simp: sl_split_def) 
+  
+lemma sl_split_eq_empty_conv[simp]: "sl_split s xs = [] \<longleftrightarrow> xs=[]"  by (auto simp: sl_split_def)
+
+lemma sl_struct_empty[simp]: "sl_struct [] = []" by (auto simp: sl_struct_def)
+lemma sl_struct_eq_empty_conv[simp]: "sl_struct xs = [] \<longleftrightarrow> xs=[]" by (auto simp: sl_struct_def)
+
+lemma sl_compat_empty[simp]: "sl_compat [] []" unfolding sl_compat_def by auto
+lemma sl_compat_empty_conv[simp]: 
+  "sl_compat [] xs\<^sub>2 \<longleftrightarrow> xs\<^sub>2 = []" 
+  "sl_compat xs\<^sub>1 [] \<longleftrightarrow> xs\<^sub>1 = []" 
+  unfolding sl_compat_def by auto
+
+
+lemma sl_join_empty[simp]: 
+  "sl_join [] xs = []"
+  "sl_join xs [] = []"
+  unfolding sl_join_def by auto
+
+lemma sl_join_eq_empty_conv[simp]: "sl_compat (sl_struct xs\<^sub>1) (sl_struct xs\<^sub>2) \<Longrightarrow> sl_join xs\<^sub>1 xs\<^sub>2 = [] \<longleftrightarrow> xs\<^sub>1=[] \<and> xs\<^sub>2=[]"  
+  unfolding sl_join_def
+  by auto
+  
+lemma sl_indexes_empty[simp]: "sl_indexes [] = {}"
+  unfolding sl_indexes_def by auto
+  
+  
+  
 lemma sl_indexes_of_list[simp]: "sl_indexes' (sl_of_list xs) = {0..<length xs}"
   unfolding sl_indexes_def sl_struct_def sl_of_list_def by auto
 
@@ -146,13 +190,6 @@ lemma sl_put_split: "i\<in>s \<Longrightarrow> sl_put (sl_split s xs) i x = sl_s
   by (auto simp: nth_list_update intro: nth_equalityI)
   
 
-lemma nth_map2: "\<lbrakk> i<length xs; i<length ys \<rbrakk> \<Longrightarrow> map2 f xs ys ! i = f (xs!i) (ys!i)" by simp
-
-lemma map2_update1: "map2 f (xs[i:=x]) ys = (map2 f xs ys)[i := f x (ys!i)]"
-  by (metis list_update_id map_update old.prod.case zip_update)
-
-lemma map2_update2: "map2 f xs (ys[i:=y]) = (map2 f xs ys)[i := f (xs!i) y]"
-  by (metis list_update_id map_update old.prod.case zip_update)
     
   
 lemma sl_get_join: "sl_compat (sl_struct xs) (sl_struct ys) \<Longrightarrow> i<length ys \<Longrightarrow> sl_get (sl_join xs ys) i = (if i\<in>sl_indexes' xs then sl_get xs i else sl_get ys i)"
@@ -195,8 +232,102 @@ lemma sl_get_complete[simp]: "sl_complete (sl_struct xs) \<Longrightarrow> sl_ge
   unfolding sl_complete_def sl_struct_def sl_of_list_def sl_get_def list_of_sl_def
   apply (cases "i<length xs")  
   by (simp_all add: nth_undefined)
+
+lemma list_eq_iff_sl_eq: "xs=xs' 
+  \<longleftrightarrow> (length xs = length xs' \<and> sl_indexes' xs = sl_indexes' xs' \<and> (\<forall>i\<in>sl_indexes' xs'. sl_get xs i = sl_get xs' i))"
+  apply (rule iffI)
+  apply (auto; fail)
+  apply (clarsimp simp: sl_indexes_alt sl_get_def list_eq_iff_nth_eq)
+  by (smt (verit) mem_Collect_eq option.exhaust_sel option.sel)
   
   
+lemma sl_join_split_eq: "sl_join (sl_split ls xs) (sl_split (-ls) xs) = xs"  
+  apply (auto simp: list_eq_iff_sl_eq sl_compat_splitI sl_indexes_split )
+  apply (subst sl_get_join)
+  apply (simp add: sl_compat_splitI; fail)
+  apply (auto dest: sl_indexes_lengthD; fail) []
+  apply (auto simp: sl_get_split sl_indexes_split)
+  done
+  
+lemma sl_put_empty_iff[simp]: "sl_put xs i x = [] \<longleftrightarrow> xs=[]"  
+  unfolding sl_put_def by auto
+
+
+lemma sl_get_put[simp]: "i\<in>sl_indexes' xs \<Longrightarrow> sl_get (sl_put xs i x) i = x"  
+  unfolding sl_get_def sl_put_def
+  by (auto dest: sl_indexes_lengthD)
+
+lemma sl_get_put_indep[simp]: "i\<noteq>j \<Longrightarrow> sl_get (sl_put xs i x) j = sl_get xs j"  
+  unfolding sl_get_def sl_put_def
+  by (auto)
+
+lemma sl_put_get[simp]: "i\<in>sl_indexes' xs \<Longrightarrow> sl_put xs i (sl_get xs i) = xs"  
+  unfolding sl_get_def sl_put_def sl_indexes_alt
+  by auto
+    
+definition "sl_split1' b x \<equiv> if b then x else None"  
+lemma sl_split1'_simp[simp]:
+  "sl_split1' True x = x"
+  "sl_split1' False x = None"
+  "sl_split1' b None = None"
+  unfolding sl_split1'_def by auto
+
+      
+lemma sl_split_snoc: "sl_split ls (xs@[x]) = sl_split ls xs @ [ sl_split1' (length xs \<in> ls) x]"  
+  unfolding sl_split_def
+  by auto
+  
+lemma sl_struct_Cons[simp]: "sl_struct (x#xs) = (x=None)#sl_struct xs"
+  by (auto simp: sl_struct_def)
+
+
+lemma sl_compat_Cons[simp]: "sl_compat (x#xs) (y#ys) \<longleftrightarrow> (x\<or>y) \<and> sl_compat xs ys"  
+  unfolding sl_compat_def
+  by simp
+      
+lemma sl_join_Cons[simp]: "sl_join (x#xs) (y#ys) = join_option x y # sl_join xs ys"  
+  unfolding sl_join_def by simp
+  
+lemma sl_indexes_finite[simp, intro!]: "finite (sl_indexes s)" by (auto simp: sl_indexes_def)
+
+lemma sl_struct_join_split: "sl_struct_join (sl_struct_split I s) (sl_struct_split (-I) s) = s"
+  unfolding sl_struct_join_def sl_struct_split_def
+  by (auto simp: map2_map_conv map_nth) 
+
+(*
+lemma sl_join_split_eq: "sl_join (sl_split s xs) (sl_split (-s) xs) = xs"  
+  unfolding sl_join_def sl_split_def 
+  apply (rewrite at "_ = \<hole>" map_nth[symmetric])
+  by (auto simp: map2_map_conv)
+*)  
+  
+lemma mset_of_list_permut: "mset xs = mset (sl_of_list xs\<^sub>0) \<Longrightarrow> mset (list_of_sl xs) = mset xs\<^sub>0" 
+  unfolding sl_of_list_def list_of_sl_def
+  by (simp add: mset_map_id)
+
+lemma length_sl_put[simp]: "length (sl_put xs i x) = length xs" unfolding sl_put_def by auto
+
+
+lemma sl_swap_aux: "\<lbrakk>i \<in> sl_indexes' xs; j \<in> sl_indexes' xs\<rbrakk> 
+  \<Longrightarrow> sl_put (sl_put xs i (sl_get xs j)) j (sl_get xs i) = swap xs i j"
+  by (auto simp add: list_eq_iff_nth_eq sl_put_def sl_get_def sl_indexes_alt swap_def)
+  
+  
+  
+(* TODO: Move *)  
+lemma sl_struct_swap[simp]: "\<lbrakk> i\<in>sl_indexes' xs; j\<in>sl_indexes' xs \<rbrakk> \<Longrightarrow> sl_struct (swap xs i j) = sl_struct xs"
+  by (simp flip: sl_swap_aux)
+  
+  
+lemma sl_get_swap_iff: "\<lbrakk> i\<in>sl_indexes' xs; j\<in>sl_indexes' xs \<rbrakk> \<Longrightarrow> sl_get (swap xs i j) k = (if k=i then sl_get xs j else if k=j then sl_get xs i else sl_get xs k)"  
+  by (auto simp add: sl_get_def swap_nth dest!: sl_indexes_lengthD)
+  
+lemma sl_get_swap_other: "\<lbrakk>k\<noteq>i; k\<noteq>j\<rbrakk> \<Longrightarrow> sl_get (swap xs i j) k = sl_get xs k"  
+  by (simp add: sl_get_def swap_def)
+
+  
+
+
 lemma slcompat_None_lower_bound:
   assumes "sl_compat (sl_struct xs\<^sub>1) (sl_struct xs\<^sub>2)"  
   shows "replicate_mset (length xs\<^sub>1) None \<subseteq># mset xs\<^sub>1 + mset xs\<^sub>2"  
@@ -228,7 +359,51 @@ lemma mset_join_idxs_eq:
     subgoal by (metis add_mset_add_single subset_mset.add_diff_assoc2)
     done
   done
+
   
+(* TODO: Move *)
+lemma fold_is_None': "(=)None = is_None" by auto
+
+lemma sl_struct_param[param]: "(sl_struct,sl_struct) \<in> \<langle>\<langle>A\<rangle>option_rel\<rangle>list_rel \<rightarrow> \<langle>bool_rel\<rangle>list_rel"  
+  unfolding sl_struct_def fold_is_None'
+  by parametricity
+  
+lemma sl_indexes_param[param]: "(sl_indexes, sl_indexes) \<in> \<langle>bool_rel\<rangle>list_rel \<rightarrow> \<langle>nat_rel\<rangle>set_rel" by simp
+
+lemma sl_split_param[param]: "(sl_split,sl_split) \<in> \<langle>nat_rel\<rangle>set_rel \<rightarrow> \<langle>\<langle>A\<rangle>option_rel\<rangle>list_rel \<rightarrow> \<langle>\<langle>A\<rangle>option_rel\<rangle>list_rel"
+  unfolding sl_split_def
+  apply parametricity
+  by auto
+
+lemma join_option_param[param]: "(join_option, join_option) \<in> \<langle>A\<rangle>option_rel \<rightarrow> \<langle>A\<rangle>option_rel \<rightarrow> \<langle>A\<rangle>option_rel"
+  by (auto simp: option_rel_def)
+
+lemma sl_join_param[param]: "(sl_join, sl_join) \<in> \<langle>\<langle>A\<rangle>option_rel\<rangle>list_rel \<rightarrow> \<langle>\<langle>A\<rangle>option_rel\<rangle>list_rel \<rightarrow> \<langle>\<langle>A\<rangle>option_rel\<rangle>list_rel"  
+  unfolding sl_join_def
+  by parametricity
+  
+lemma sl_complete_sl_of_list_of_sl[simp]: "sl_complete (sl_struct xs) \<Longrightarrow> sl_of_list (list_of_sl xs) = xs"
+  unfolding sl_of_list_def list_of_sl_def sl_complete_def
+  apply (induction xs)
+  by auto
+  
+  
+  
+subsection \<open>Sepref ADT Setup\<close>  
+sepref_decl_op slist_swap: "swap:: _ option list \<Rightarrow> _ "
+  :: "[\<lambda>((l,i),j). i\<in>sl_indexes' l \<and> j\<in>sl_indexes' l]\<^sub>f (\<langle>\<langle>A\<rangle>option_rel\<rangle>list_rel \<times>\<^sub>r nat_rel) \<times>\<^sub>r nat_rel \<rightarrow> \<langle>\<langle>A\<rangle>option_rel\<rangle>list_rel" 
+  apply rule
+  apply (clarsimp dest!: sl_indexes_lengthD)
+  apply parametricity
+  by auto
+
+sepref_decl_op sl_of_list :: "\<langle>Id::'a rel\<rangle>list_rel \<rightarrow> \<langle>\<langle>Id::'a rel\<rangle>option_rel\<rangle>list_rel" . 
+  
+sepref_decl_op list_of_sl :: "[\<lambda>xs. sl_complete (sl_struct xs) ]\<^sub>f \<langle>\<langle>Id::'a rel\<rangle>option_rel\<rangle>list_rel \<rightarrow> \<langle>Id::'a rel\<rangle>list_rel" by auto 
+  
+  
+    
+subsection \<open>With-Idxs Combinator\<close>  
   
 definition "WITH_IDXS ls xs m \<equiv> do {
   ASSERT (ls\<subseteq>sl_indexes' xs);
@@ -276,11 +451,6 @@ lemma WITH_IDXS_mono_flat[refine_mono]:
   by refine_mono
   
   
-find_in_thms WHILEIT in sepref_monadify_arity sepref_monadify_comb 
-
-find_theorems WHILEIT PR_CONST
-
-  
 (* Monadifier setup *)
 
 lemma WITH_IDXS_pat[def_pat_rules]:
@@ -301,32 +471,6 @@ lemma WITH_IDXS_comb[sepref_monadify_comb]:
   by simp
 
   
-(* TODO: Move *)
-lemma fold_is_None': "(=)None = is_None" by auto
-
-lemma sl_struct_param[param]: "(sl_struct,sl_struct) \<in> \<langle>\<langle>A\<rangle>option_rel\<rangle>list_rel \<rightarrow> \<langle>bool_rel\<rangle>list_rel"  
-  unfolding sl_struct_def fold_is_None'
-  by parametricity
-  
-term sl_indexes  
-
-lemma sl_indexes_param[param]: "(sl_indexes, sl_indexes) \<in> \<langle>bool_rel\<rangle>list_rel \<rightarrow> \<langle>nat_rel\<rangle>set_rel" by simp
-
-term sl_split
-
-lemma sl_split_param[param]: "(sl_split,sl_split) \<in> \<langle>nat_rel\<rangle>set_rel \<rightarrow> \<langle>\<langle>A\<rangle>option_rel\<rangle>list_rel \<rightarrow> \<langle>\<langle>A\<rangle>option_rel\<rangle>list_rel"
-  unfolding sl_split_def
-  apply parametricity
-  by auto
-
-term sl_join
-
-lemma join_option_param[param]: "(join_option, join_option) \<in> \<langle>A\<rangle>option_rel \<rightarrow> \<langle>A\<rangle>option_rel \<rightarrow> \<langle>A\<rangle>option_rel"
-  by (auto simp: option_rel_def)
-
-lemma sl_join_param[param]: "(sl_join, sl_join) \<in> \<langle>\<langle>A\<rangle>option_rel\<rangle>list_rel \<rightarrow> \<langle>\<langle>A\<rangle>option_rel\<rangle>list_rel \<rightarrow> \<langle>\<langle>A\<rangle>option_rel\<rangle>list_rel"  
-  unfolding sl_join_def
-  by parametricity
   
   
   
@@ -364,226 +508,5 @@ lemma WITH_IDXS_refine[refine]:
     apply parametricity
     by simp_all  
   done  
-  
-    
-(*  
-lemma join_option_eq_Some_iff[simp]: 
-  "join_option (Some xv) y = Some xv' \<longleftrightarrow> xv'=xv \<and> y=None"
-  "join_option x (Some yv) = Some yv' \<longleftrightarrow> yv'=yv \<and> x=None"
-  "join_option None y = Some yv' \<longleftrightarrow> y=Some yv'"
-  "join_option x None = Some xv' \<longleftrightarrow> x=Some xv'"
-  apply (cases y; auto)
-  apply (cases x; auto)
-  apply (cases y; auto)
-  apply (cases x; auto)
-  done
-
-
-lemma param_join_option[param]: "(join_option,join_option) \<in> \<langle>A\<rangle>option_rel \<rightarrow> \<langle>A\<rangle>option_rel \<rightarrow> \<langle>A\<rangle>option_rel"
-  by (auto simp: option_rel_def)
-
-
-lemma join_idxs_param[param]: "(join_idxs,join_idxs) \<in> \<langle>\<langle>A\<rangle>option_rel\<rangle>list_rel \<rightarrow> \<langle>\<langle>A\<rangle>option_rel\<rangle>list_rel \<rightarrow> \<langle>\<langle>A\<rangle>option_rel\<rangle>list_rel"
-  unfolding join_idxs_def
-  by parametricity
-
-(*
-definition "join_idxs xs\<^sub>1 xs\<^sub>2 = map (\<lambda>i. if i<length xs\<^sub>1 \<and> i<length xs\<^sub>2 then (if xs\<^sub>1!i=None then xs\<^sub>2!i else xs\<^sub>1!i) else None) [0..<length xs\<^sub>1]"
-*)
-
-lemma map_compat_split_aux: "map ((=) None \<circ> (\<lambda>i. P i ((xs @ [x]) ! i))) [0..<length xs] = map ((=) None \<circ> (\<lambda>i. P i (xs ! i))) [0..<length xs]" by simp
-
-lemma map_compat_split_aux1: "
-    (map ((=) None \<circ> (\<lambda>i. if i \<in> ls \<and> i < Suc (length xs) then (xs @ [x]) ! i else None)) [0..<length xs]) 
-  = (map ((=) None \<circ> (\<lambda>i. if i \<in> ls \<and> i < length xs then xs ! i else None)) [0..<length xs])"
-  by simp
-
-lemma map_compat_split_aux2: "
-    (map ((=) None \<circ> (\<lambda>i. if i \<in> ls \<or> Suc (length xs) \<le> i then None else (xs @ [x]) ! i)) [0..<length xs])
-  = (map ((=) None \<circ> (\<lambda>i. if i \<in> ls \<or> length xs \<le> i then None else xs ! i)) [0..<length xs])"  
-  by simp
-
-lemma slcompat_struct_split[simp]: "slcompat (slstruct (split_idxs_left ls xs)) (slstruct (split_idxs_right ls xs))"
-  unfolding slcompat_def slstruct_def split_idxs_left_def split_idxs_right_def
-  apply (induction xs rule: rev_induct)
-  apply simp
-  by (clarsimp simp: list_all2_append map_compat_split_aux1 map_compat_split_aux2)
-
-lemma "i\<in>ls \<Longrightarrow> split_idxs_left ls xs ! i = xs ! i"
-  unfolding split_idxs_left_def
-  apply (cases "i<length xs")
-  by (auto simp: nth_undefined)
-  
-lemma "i\<notin>ls \<Longrightarrow> split_idxs_right ls xs ! i = xs ! i"
-  unfolding split_idxs_right_def
-  apply (cases "i<length xs")
-  by (auto simp: nth_undefined)
-
-lemma opt_list_rel_imp_same_sl_struct: "(xs', xs) \<in> \<langle>\<langle>A\<rangle>option_rel\<rangle>list_rel \<Longrightarrow> slstruct xs' = slstruct xs"  
-  unfolding slstruct_def
-  apply (rule IdD)
-  apply (subst list_rel_id_simp[symmetric])
-  apply parametricity
-  by auto
-
-
-lemma opt_list_rel_imp_same_sl_indexes: "(xs', xs) \<in> \<langle>\<langle>A\<rangle>option_rel\<rangle>list_rel \<Longrightarrow> sl_indexes xs' = sl_indexes xs"  
-  unfolding sl_indexes_def
-  apply (auto simp: list_rel_imp_same_length)
-  apply (metis not_None_eq option_rel_simp(2) pair_in_Id_conv param_nth)
-  apply (metis not_None_eq option_rel_simp(1) pair_in_Id_conv param_nth)
-  done
-  
-  
-lemma slstruct_eq_imps: "slstruct a = slstruct b \<Longrightarrow> length a = length b \<and> sl_indexes a = sl_indexes b"  
-  unfolding slstruct_def sl_indexes_def
-  apply (auto dest: map_eq_imp_length_eq)
-  apply (metis (full_types) length_map not_Some_eq nth_map)
-  apply (metis (full_types) length_map not_Some_eq nth_map)
-  done
-  
-term split_idxs_left  
-lemma split_idxs_left_param[param]: "(split_idxs_left,split_idxs_left) \<in> \<langle>Id\<rangle>set_rel \<rightarrow> \<langle>\<langle>A\<rangle>option_rel\<rangle>list_rel \<rightarrow> \<langle>\<langle>A\<rangle>option_rel\<rangle>list_rel"
-  unfolding split_idxs_left_def
-  apply parametricity
-  by auto
-  
-lemma split_idxs_right_param[param]: "(split_idxs_right,split_idxs_right) \<in> \<langle>Id\<rangle>set_rel \<rightarrow> \<langle>\<langle>A\<rangle>option_rel\<rangle>list_rel \<rightarrow> \<langle>\<langle>A\<rangle>option_rel\<rangle>list_rel"
-  unfolding split_idxs_right_def
-  apply parametricity
-  by auto
-  
-term join_idxs
-
-lemma sl_indexes_alt: "sl_indexes xs = {i . i<length (slstruct xs) \<and> \<not>(slstruct xs)!i}"
-  unfolding sl_indexes_def slstruct_def
-  by auto
-  
-lemma length_slstruct[simp]: "length (slstruct xs) = length xs" unfolding slstruct_def by auto
-  
-lemma length_join_idxs[simp]: "length (join_idxs xs\<^sub>1 xs\<^sub>2) = min (length xs\<^sub>1) (length xs\<^sub>2)"  
-  unfolding join_idxs_def by auto
-
-lemma sl_indexes_in_range: "sl_indexes xs \<subseteq> {0..<length xs}"  
-  unfolding sl_indexes_def by auto
-  
-
-  
-lemma slcompat_alt: "slcompat (slstruct xs\<^sub>1) (slstruct xs\<^sub>2) \<longleftrightarrow> (length xs\<^sub>1 = length xs\<^sub>2 \<and> sl_indexes xs\<^sub>1 \<inter> sl_indexes xs\<^sub>2 = {})"  
-  unfolding sl_indexes_alt slcompat_def
-  by (auto 0 2 dest: list_all2_lengthD simp: list_all2_conv_all_nth)
-  
-lemma in_sl_indexes_iff: "i \<in> sl_indexes xs \<longleftrightarrow> (i<length xs \<and> xs!i\<noteq>None)"  
-  unfolding sl_indexes_def by auto
-  
-lemma join_idxs_nth: "\<lbrakk> i<length xs\<^sub>1; i<length xs\<^sub>2 \<rbrakk> \<Longrightarrow> join_idxs xs\<^sub>1 xs\<^sub>2 ! i = join_option (xs\<^sub>1!i) (xs\<^sub>2!i)"  
-  unfolding join_idxs_def
-  by (auto simp: )
-  
-  
-lemma slstruct_empty[simp]: "slstruct [] = []" unfolding slstruct_def by auto 
-lemma slstruct_Cons[simp]: "slstruct (x#xs) = (x=None)#slstruct xs" unfolding slstruct_def by auto 
-lemma slstruct_append[simp]: "slstruct (xs@ys) = slstruct xs @ slstruct ys" unfolding slstruct_def by auto 
-  
-lemma slcompat_empty[simp]: "slcompat [] []"
-  unfolding slcompat_def by auto
-  
-lemma slcompat_Cons[simp]: "slcompat (x#xs) (y#ys) \<longleftrightarrow> (x\<or>y) \<and> slcompat xs ys"  
-  unfolding slcompat_def by auto
-
-    
-lemma slcompat_Snoc[simp]: "slcompat (xs@[x]) (ys@[y]) \<longleftrightarrow> slcompat xs ys \<and> (x\<or>y)"  
-  unfolding slcompat_def 
-  by (auto simp: list_all2_append2)
-  
-    
-
-lemma join_idxs_empty[simp]: "join_idxs [] [] = []"
-  unfolding join_idxs_def by auto
-
-lemma join_idxs_Cons[simp]: "join_idxs (x#xs) (y#ys) = join_option x y # join_idxs xs ys"
-  unfolding join_idxs_def
-  by auto
-  
-lemma join_idxs_append[simp]: "length xs = length ys \<Longrightarrow> join_idxs (xs@xs') (ys@ys') = join_idxs xs ys @ join_idxs xs' ys'"
-  unfolding join_idxs_def
-  by auto
-
-
-lemma slcompat_None_lower_bound:
-  assumes "slcompat (slstruct xs\<^sub>1) (slstruct xs\<^sub>2)"  
-  shows "replicate_mset (length xs\<^sub>1) None \<subseteq># mset xs\<^sub>1 + mset xs\<^sub>2"  
-proof -
-  from assms have "length xs\<^sub>1 = length xs\<^sub>2" by (auto simp: slcompat_alt)
-  then show ?thesis using assms
-    apply (induction xs\<^sub>1 xs\<^sub>2 rule: list_induct2)
-    apply simp
-    apply (clarsimp)
-    by (meson mset_le_add_mset_decr_left1 mset_subset_eq_add_mset_cancel)
-qed      
-  
-lemma mset_join_idxs_eq:
-  assumes "slcompat (slstruct xs\<^sub>1) (slstruct xs\<^sub>2)"  
-  shows "mset (join_idxs xs\<^sub>1 xs\<^sub>2) = mset xs\<^sub>1 + mset xs\<^sub>2 - replicate_mset (length xs\<^sub>1) None"
-proof -
-  from assms have "length xs\<^sub>1 = length xs\<^sub>2" by (auto simp: slcompat_alt)
-  then show ?thesis using assms
-    apply (induction xs\<^sub>1 xs\<^sub>2 rule: list_induct2)
-    apply simp
-    apply (clarsimp;safe; clarsimp)
-    subgoal
-      apply (subst subset_mset.add_diff_assoc[of _ _ "{#_#}", simplified])
-      apply (drule slcompat_None_lower_bound)
-      by auto
-    subgoal
-      apply (subst subset_mset.add_diff_assoc[of _ _ "{#_#}", simplified])
-      apply (drule slcompat_None_lower_bound)
-      by auto
-    done  
-qed    
-    
-
-lemma split_idxs_length[simp]:
-  "length (split_idxs_left s xs) = length xs"
-  "length (split_idxs_right s xs) = length xs"
-  unfolding split_idxs_left_def split_idxs_right_def
-  by auto
-  
-lemma sl_indexes_split_left[simp]: "sl_indexes (split_idxs_left s xs) = s \<inter> sl_indexes xs"
-  unfolding sl_indexes_def split_idxs_left_def
-  by (auto split: if_splits)
-  
-lemma sl_indexes_split_right[simp]: "sl_indexes (split_idxs_right s xs) = sl_indexes xs - s"
-  unfolding sl_indexes_def split_idxs_right_def
-  by (auto split: if_splits)
-  
-
-lemma slstruct_join_idxs[simp]:
-  shows "slstruct (join_idxs xs ys) = map2 (=) (slstruct xs) (slstruct ys)"
-  apply (induction xs arbitrary: ys)
-  apply (simp add: join_idxs_def)
-  subgoal for a xs ys
-    apply (cases ys)
-    by (auto simp: join_idxs_def)
-  done
-  
-  
-  
-lemma slstruct_split_recombine:
-  "map2 (=) (slstruct (split_idxs_left s xs)) (slstruct (split_idxs_right s xs)) = slstruct xs"  
-  unfolding slstruct_def split_idxs_right_def split_idxs_left_def fun_eq_iff
-  apply (simp add: map2_map_conv)
-  apply (rewrite in "_ = \<hole>" map_by_map_idx)
-  by simp
-  
-
-lemma join_split_idxs: "join_idxs (split_idxs_left s xs) (split_idxs_right s xs) = xs"
-  unfolding join_idxs_def split_idxs_left_def split_idxs_right_def
-  apply (simp add: map2_map_conv)
-  apply (rewrite at "_ = \<hole>" list.map_id[symmetric])
-  apply (rewrite in "_ = \<hole>" map_by_map_idx)
-  by simp
-*)  
-
 
 end
