thys/examples/sorting/Sorting_Guarded_Partition.thy
@@ -1,6 +1,20 @@
 theory Sorting_Guarded_Partition
 imports Sorting_Quicksort_Scheme
 begin
+
+(* TODO: Move *)
+lemma slice_update_outside[simp]: "i\<notin>{l..<h} \<Longrightarrow> slice l h (xs[i:=x]) = slice l h xs"
+  unfolding Misc.slice_def
+  apply auto
+  by (metis drop_take leI take_update_cancel)
+
+lemma slice_eq_mset_upd_outside: "slice_eq_mset l h xs xs' \<Longrightarrow> i\<notin>{l..<h} \<Longrightarrow> i<length xs' \<Longrightarrow> slice_eq_mset l h (xs[i:=x]) (xs'[i:=x])"
+  unfolding slice_eq_mset_def
+  apply (auto simp: drop_update_swap not_le)
+  by (metis drop_update_cancel drop_update_swap leI)
+
+
+
   
 hide_const (open) Transcendental.pi \<comment> \<open>\<open>pi\<close> is the implementation of \<open>p\<close>, not some constant related to a circle ;)\<close>
 
@@ -288,18 +302,6 @@ definition "qsg_partition_wrapper li hi p xs \<equiv> do {
 }"
 
 
-(* TODO: Move *)
-lemma slice_update_outside[simp]: "i\<notin>{l..<h} \<Longrightarrow> slice l h (xs[i:=x]) = slice l h xs"
-  unfolding Misc.slice_def
-  apply auto
-  by (metis drop_take leI take_update_cancel)
-
-lemma slice_eq_mset_upd_outside: "slice_eq_mset l h xs xs' \<Longrightarrow> i\<notin>{l..<h} \<Longrightarrow> i<length xs' \<Longrightarrow> slice_eq_mset l h (xs[i:=x]) (xs'[i:=x])"
-  unfolding slice_eq_mset_def
-  apply (auto simp: drop_update_swap not_le)
-  by (metis drop_update_cancel drop_update_swap leI)
-
-
 lemma qsg_partition_correct: "li+1<hi \<Longrightarrow> qsg_partition li hi p xs \<le> gpartition_SPEC li hi p xs"
   unfolding qsg_partition_def gpartition_SPEC_def
   apply (refine_vcg qsg_partition_aux_correct[THEN order_trans])
@@ -382,17 +384,6 @@ lemma qsg_partition_correct: "li+1<hi \<Longrightarrow> qsg_partition li hi p xs
   
 end  
   
-
-(* TODO: Move to Sorting-Setup *)
-
-find_theorems GEN_ALGO
-
-
-  
-term "GEN_ALGO"
-
-term mop_list_copy
-
 
 context sort_impl_context begin
 
@@ -540,206 +531,6 @@ lemmas qsg_partition_wrapper_impl'_hnr[sepref_fr_rules] = qsg_partition_wrapper_
   
 
 end
-
-(*
-  skip for now, as we won't yet be able to distribute the comparator data over many threads!
-
-subsection \<open>Parameterization\<close>
-
-context parameterized_weak_ordering begin
-  thm WO.qsg_next_l_def
-
-  definition qsg_next_l_param :: "'cparam \<Rightarrow> 'a list \<Rightarrow> nat \<Rightarrow> nat \<Rightarrow> nat \<Rightarrow> nat nres" where            
-    "qsg_next_l_param cparam xs pi li hi \<equiv> doN {
-      monadic_WHILEIT (\<lambda>_. True) 
-        (\<lambda>li. doN {ASSERT (li\<noteq>pi); pcmp_idxs2 cparam xs li pi}) 
-        (\<lambda>li. doN {ASSERT (li<hi); RETURN (li + 1)}) li
-    }"  
-  
-  lemma qsg_next_l_param_refine[refine]: "\<lbrakk>
-    (xs',xs)\<in>cdom_list_rel cparam; (p',p)\<in>Id; (i',i)\<in>Id; (h',h)\<in>Id
-  \<rbrakk> \<Longrightarrow> qsg_next_l_param cparam xs' p' i' h' \<le>\<Down>nat_rel (WO.ungrd_qsg_next_l_spec cparam xs p i h)"
-  proof (goal_cases)
-    case 1
-    then have "qsg_next_l_param cparam xs' p' i' h' \<le>\<Down>nat_rel (WO.qsg_next_l cparam xs p i h)" 
-      unfolding qsg_next_l_param_def WO.qsg_next_l_def
-      apply refine_rcg
-      by auto
-    also note WO.qsg_next_l_refine[param_fo, OF IdI IdI IdI IdI, of cparam xs p i h, THEN nres_relD]
-    finally show ?case unfolding PR_CONST_def .
-  qed 
-  
-    
-  definition qsg_next_h_param :: "'cparam \<Rightarrow> 'a list \<Rightarrow> nat \<Rightarrow> nat \<Rightarrow> nat nres" where
-    "qsg_next_h_param cparam xs pi hi \<equiv> doN {
-      ASSERT (hi>0);
-      let hi = hi - 1;
-      ASSERT (hi<length xs);
-      monadic_WHILEIT (\<lambda>_. True)
-        (\<lambda>hi. doN {ASSERT(pi\<noteq>hi); pcmp_idxs2 cparam xs pi hi}) 
-        (\<lambda>hi. doN { ASSERT(hi>0); RETURN (hi - 1)}) hi
-    }"  
-
-  lemma qsg_next_h_param_refine[refine]: "\<lbrakk>
-    (xs',xs)\<in>cdom_list_rel cparam; (p',p)\<in>Id; (h',h)\<in>Id
-  \<rbrakk> \<Longrightarrow> qsg_next_h_param cparam xs' p' h' \<le>\<Down>nat_rel (WO.ungrd_qsg_next_h_spec cparam xs p h)"      
-  proof goal_cases
-    case 1
-    then have "qsg_next_h_param cparam xs' p' h' \<le>\<Down>nat_rel (WO.qsg_next_h cparam xs p h)"
-      unfolding qsg_next_h_param_def WO.qsg_next_h_def
-      apply refine_rcg
-      by (auto simp: cdom_list_rel_alt in_br_conv)
-    also note WO.qsg_next_h_refine[param_fo, THEN nres_relD]
-    finally show ?thesis by simp 
-  qed    
-    
-  definition "qsg_partition_param cparam li\<^sub>0 hi\<^sub>0 pi xs\<^sub>0 \<equiv> doN {
-    ASSERT (pi < li\<^sub>0 \<and> li\<^sub>0<hi\<^sub>0 \<and> hi\<^sub>0\<le>length xs\<^sub>0);
-    
-    \<comment> \<open>Initialize\<close>
-    li \<leftarrow> qsg_next_l_param cparam xs\<^sub>0 pi li\<^sub>0 hi\<^sub>0;
-    hi \<leftarrow> qsg_next_h_param cparam xs\<^sub>0 pi hi\<^sub>0;
-    
-    ASSERT (li\<^sub>0\<le>hi);
-    
-    (xs,li,hi) \<leftarrow> WHILEIT 
-      (\<lambda>_. True)
-      (\<lambda>(xs,li,hi). li<hi) 
-      (\<lambda>(xs,li,hi). doN {
-        ASSERT(li<hi \<and> li<length xs \<and> hi<length xs \<and> li\<noteq>hi);
-        xs \<leftarrow> mop_list_swap xs li hi;
-        let li = li + 1;
-        li \<leftarrow> qsg_next_l_param cparam xs pi li hi\<^sub>0;
-        hi \<leftarrow> qsg_next_h_param cparam xs pi hi;
-        RETURN (xs,li,hi)
-      }) 
-      (xs\<^sub>0,li,hi);
-    
-    RETURN (xs,li)
-  }"  
-
-  lemma qsg_partition_param_refine[refine]: "\<lbrakk>
-    (li',li)\<in>Id; (hi',hi)\<in>Id; (pi',pi)\<in>Id; (xs',xs)\<in>cdom_list_rel cparam
-  \<rbrakk> \<Longrightarrow> qsg_partition_param cparam li' hi' pi' xs' 
-    \<le> \<Down>(cdom_list_rel cparam \<times>\<^sub>r nat_rel) (WO.qsg_partition cparam li hi pi xs)" 
-    unfolding qsg_partition_param_def WO.qsg_partition_def
-    supply [refine_dref_RELATES] = RELATESI[of "cdom_list_rel cparam"]
-    apply refine_rcg
-    apply refine_dref_type
-    apply (auto simp: cdom_list_rel_alt in_br_conv)
-    done
-
- definition "move_median_to_first_param cparam ri ai bi ci (xs::'a list) = doN {
-    ASSERT (ai \<noteq> bi \<and> ai \<noteq> ci \<and> bi \<noteq> ci \<and> ri \<noteq> ai \<and> ri \<noteq> bi \<and> ri \<noteq> ci);
-    if\<^sub>N pcmp_idxs2 cparam xs ai bi then (
-      if\<^sub>N pcmp_idxs2 cparam xs bi ci then
-        mop_list_swap xs ri bi
-      else if\<^sub>N pcmp_idxs2 cparam xs ai ci then
-        mop_list_swap xs ri ci
-      else 
-        mop_list_swap xs ri ai
-    ) 
-    else if\<^sub>N pcmp_idxs2 cparam xs ai ci then
-      mop_list_swap xs ri ai
-    else if\<^sub>N pcmp_idxs2 cparam xs bi ci then 
-      mop_list_swap xs ri ci
-    else 
-      mop_list_swap xs ri bi
-  }"
-
-  
-  (* TODO:Move *)
-  lemma mop_list_swap_cdom_refine[refine]: "\<lbrakk>
-    (xs',xs)\<in>cdom_list_rel cparam; (i',i)\<in>Id; (j',j)\<in>Id
-  \<rbrakk> \<Longrightarrow> mop_list_swap xs' i' j' \<le> \<Down> (cdom_list_rel cparam) (mop_list_swap xs i j)"
-    apply simp
-    apply refine_rcg
-    apply (clarsimp_all simp: cdom_list_rel_def list_rel_imp_same_length)
-    apply (parametricity)
-    by auto
-  
-  lemma move_median_to_first_param_refine[refine]: "\<lbrakk>
-    (ri',ri)\<in>Id; (ai',ai)\<in>Id; (bi',bi)\<in>Id; (ci',ci)\<in>Id; (xs',xs)\<in>cdom_list_rel cparam 
-  \<rbrakk> \<Longrightarrow> move_median_to_first_param cparam ri' ai' bi' ci' xs' 
-    \<le> \<Down>(cdom_list_rel cparam) (WO.move_median_to_first cparam ri ai bi ci xs)"
-    unfolding move_median_to_first_param_def WO.move_median_to_first_alt
-    apply refine_rcg  
-    by auto  
-    
-  definition "partition_pivot_param cparam xs\<^sub>0 l h \<equiv> doN {
-    ASSERT (l\<le>h \<and> h\<le>length xs\<^sub>0 \<and> h-l\<ge>4);
-    let m = l + (h-l) div 2;
-    xs\<^sub>1 \<leftarrow> move_median_to_first_param cparam l (l+1) m (h-1) xs\<^sub>0;
-    ASSERT (l<length xs\<^sub>1 \<and> length xs\<^sub>1 = length xs\<^sub>0);
-    (xs,m) \<leftarrow> qsg_partition_param cparam (l+1) h l xs\<^sub>1;
-  
-    RETURN (xs,m)
-  }"
-
-  lemma partition_pivot_param_refine[refine]: "\<lbrakk> (xs',xs)\<in>cdom_list_rel cparam; (l',l)\<in>Id; (h',h)\<in>Id
-    \<rbrakk> \<Longrightarrow> partition_pivot_param cparam xs' l' h' 
-        \<le> \<Down>(cdom_list_rel cparam \<times>\<^sub>r nat_rel) (WO.partition_pivot cparam xs l h)"
-    unfolding partition_pivot_param_def WO.partition_pivot_def   
-    apply refine_rcg
-    apply (auto simp: cdom_list_rel_alt in_br_conv)
-    done    
-        
-end
-
-
-context parameterized_sort_impl_context begin
-
-  (* TODO: Move *)
-  abbreviation "arr_assn \<equiv> wo_assn"
-
-  
-sepref_register qsg_next_l_param qsg_next_h_param
-
-(* TODO: We can get rid of the length xs restriction: the stopper element will always lie within <h, which is size_t representable! *)
-sepref_def qsg_next_l_impl [llvm_inline] is "uncurry4 (PR_CONST qsg_next_l_param)" 
-  :: "cparam_assn\<^sup>k *\<^sub>a (arr_assn)\<^sup>k *\<^sub>a size_assn\<^sup>k *\<^sub>a size_assn\<^sup>k *\<^sub>a size_assn\<^sup>k \<rightarrow>\<^sub>a size_assn"
-  unfolding qsg_next_l_param_def PR_CONST_def
-  apply (annot_snat_const "TYPE(size_t)")
-  by sepref
- 
-sepref_def qsg_next_h_impl [llvm_inline] is "uncurry3 (PR_CONST qsg_next_h_param)" :: "cparam_assn\<^sup>k *\<^sub>a (arr_assn)\<^sup>k *\<^sub>a size_assn\<^sup>k *\<^sub>a size_assn\<^sup>k \<rightarrow>\<^sub>a size_assn"
-  unfolding qsg_next_h_param_def PR_CONST_def
-  apply (annot_snat_const "TYPE(size_t)")
-  by sepref
-  
-                        
-sepref_register qsg_partition_param  
-sepref_def qsg_partition_impl is "uncurry4 (PR_CONST qsg_partition_param)" 
-  :: "[\<lambda>_. True]\<^sub>c cparam_assn\<^sup>k *\<^sub>a size_assn\<^sup>k *\<^sub>a size_assn\<^sup>k *\<^sub>a size_assn\<^sup>k *\<^sub>a (arr_assn)\<^sup>d 
-    \<rightarrow> arr_assn \<times>\<^sub>a size_assn [\<lambda>((((_,_),_),_),ai) (r,_). r=ai]\<^sub>c"
-  unfolding qsg_partition_param_def PR_CONST_def
-  apply (annot_snat_const "TYPE(size_t)")
-  supply [dest] = slice_eq_mset_eq_length
-  by sepref
-
-sepref_register move_median_to_first_param
-
-sepref_def move_median_to_first_param_impl (*[llvm_inline] *)
-  is "uncurry5 (PR_CONST move_median_to_first_param)" 
-  :: "[\<lambda>_. True]\<^sub>c cparam_assn\<^sup>k *\<^sub>a size_assn\<^sup>k *\<^sub>a size_assn\<^sup>k *\<^sub>a size_assn\<^sup>k *\<^sub>a size_assn\<^sup>k *\<^sub>a (arr_assn)\<^sup>d 
-    \<rightarrow> arr_assn [\<lambda>(((((_,_),_),_),_),ai) r. r=ai]\<^sub>c"
-  unfolding move_median_to_first_param_def PR_CONST_def
-  by sepref  
-  
-  
-sepref_register partition_pivot_param  
-sepref_def partition_pivot_impl (*[llvm_inline] *)
-  is "uncurry3 (PR_CONST partition_pivot_param)" 
-  :: "[\<lambda>_. True]\<^sub>c cparam_assn\<^sup>k *\<^sub>a arr_assn\<^sup>d *\<^sub>a size_assn\<^sup>k *\<^sub>a size_assn\<^sup>k 
-    \<rightarrow> arr_assn \<times>\<^sub>a size_assn [\<lambda>(((_,ai),_),_) (r,_). r=ai]\<^sub>c"
-  unfolding partition_pivot_param_def PR_CONST_def    
-  apply (annot_snat_const "TYPE(size_t)")
-  by sepref
-  
-
-end
-
-*)
 
 end                           
 
