thys/examples/sorting/Sorting_Parsort.thy
@@ -7,118 +7,120 @@ begin
 
 context weak_ordering begin
 
-    subsection \<open>Abstract Algorithm\<close>
-    text \<open>We use a few straightforward refinement steps to develop the abstract parallel 
-      quicksort algorithm\<close>
-            
-    definition bad_partition :: "nat \<Rightarrow> nat \<Rightarrow> bool nres" where 
-    "bad_partition m n \<equiv> do {
-      ASSERT (m\<le>n);
-      RETURN (m < n div 8 \<or> n-m < n div 8)
-    }"
-  
-    lemma bad_partition_triv: "m\<le>n \<Longrightarrow> bad_partition m n \<le> SPEC (\<lambda>_. True)"
-      unfolding bad_partition_def
-      apply refine_vcg
-      by simp
-    
-    abbreviation "par_sort_seq_threshold::nat \<equiv> 100000"  
-    abbreviation "ppar_chunk_size::nat \<equiv> 1000000"  
-      
-    definition "par_sort_aux xs d \<equiv> RECT (\<lambda>par_sort_aux (xs,d::nat). doN {
-      let n = length xs;
-      if d=0 \<or> n<par_sort_seq_threshold then
-        slice_sort_spec (\<^bold><) xs 0 n
-      else doN {
-        (xs',m) \<leftarrow> partition3_spec xs 0 n;
-        bad \<leftarrow> bad_partition m n;
-        
-        ASSERT (length xs' = length xs);
-        (_,xs'') \<leftarrow> WITH_SPLIT m xs' (\<lambda>xs\<^sub>1 xs\<^sub>2. doN {
-          ASSERT (length xs' = length xs\<^sub>1 + length xs\<^sub>2);
-          (xs\<^sub>1',xs\<^sub>2') \<leftarrow> if bad then doN {
-            xs\<^sub>1' \<leftarrow> par_sort_aux (xs\<^sub>1,d-1);
-            ASSERT (length xs\<^sub>1' = length xs\<^sub>1);
-            xs\<^sub>2' \<leftarrow> par_sort_aux (xs\<^sub>2,d-1);
-            ASSERT (length xs\<^sub>2' = length xs\<^sub>2);
-            RETURN (xs\<^sub>1',xs\<^sub>2')
-          } else doN {
-            xs\<^sub>1' \<leftarrow> par_sort_aux (xs\<^sub>1,d-1);
-            ASSERT (length xs\<^sub>1' = length xs\<^sub>1);
-            xs\<^sub>2' \<leftarrow> par_sort_aux (xs\<^sub>2,d-1);
-            ASSERT (length xs\<^sub>2' = length xs\<^sub>2);
-            RETURN (xs\<^sub>1',xs\<^sub>2')
-          };
-          RETURN ((),xs\<^sub>1',xs\<^sub>2')
-        });
-        RETURN xs''
-      }
-    }) (xs,d)"
-    
-    
-    lemma par_sort_aux_correct: "par_sort_aux xs d \<le> slice_sort_spec (\<^bold><) xs 0 (length xs)"
-      unfolding par_sort_aux_def 
-      apply (subst if_cancel)
-      apply (refine_vcg RECT_rule_arb[where V="measure (\<lambda>(_,d). d)" and pre="\<lambda>xss (xs,d). xss=xs"])
-      apply simp_all [2]
-      unfolding slice_sort_spec_def partition3_spec_def
-      apply (refine_vcg bad_partition_triv)
-      apply simp_all 
-      apply (meson slice_eq_mset_all slice_eq_mset_def)
-      apply (rule order_trans) apply (rprems)
-      apply simp
-      apply simp
-      apply refine_vcg
-      apply (clarsimp)
-      apply (rule order_trans) apply (rprems)
-      apply simp
-      apply simp
-      apply refine_vcg
-      apply (clarsimp_all)
-      subgoal for xs' xs\<^sub>2' xs\<^sub>1 xs\<^sub>2 xc x1b
-        
-        unfolding sort_spec_def slice_eq_mset_def slice_LT_def
-        apply (auto simp: slice_complete' sorted_wrt_append le_by_lt slice_append1' slice_append2')
-        by (metis set_mset_mset)
-      done
-      
-    text \<open>Introducing explicit parameter for list length\<close>  
-    definition "par_sort_aux2 xs n d \<equiv> RECT (\<lambda>par_sort_aux (xs,n,d::nat). doN {
-      ASSERT (n = length xs);
-      if d=0 \<or> n<par_sort_seq_threshold then
-        slice_sort_spec (\<^bold><) xs 0 n
-      else doN {
-        (xs,m) \<leftarrow> partition3_spec xs 0 n;
-        bad \<leftarrow> bad_partition m n;
-        (_,xs) \<leftarrow> WITH_SPLIT m xs (\<lambda>xs\<^sub>1 xs\<^sub>2. doN {
-          ASSERT (length xs\<^sub>2 = length xs - m);
-          ASSERT (n\<ge>m);
-          (xs\<^sub>1,xs\<^sub>2) \<leftarrow> if bad then doN {
-            xs\<^sub>1 \<leftarrow> par_sort_aux (xs\<^sub>1,m,d-1);
-            xs\<^sub>2 \<leftarrow> par_sort_aux (xs\<^sub>2,n-m,d-1);
-            RETURN (xs\<^sub>1,xs\<^sub>2)
-          } else doN {
-            nres_par par_sort_aux par_sort_aux (xs\<^sub>1,m,d-1) (xs\<^sub>2,n-m,d-1)
-          };
-          RETURN ((),xs\<^sub>1,xs\<^sub>2)
-        });
-        RETURN xs
-      }
-    }) (xs,n,d)"
+  subsection \<open>Abstract Algorithm\<close>
+  text \<open>We use a few straightforward refinement steps to develop the abstract parallel 
+    quicksort algorithm\<close>
+          
+  definition bad_partition :: "nat \<Rightarrow> nat \<Rightarrow> bool nres" where 
+  "bad_partition m n \<equiv> do {
+    ASSERT (m\<le>n);
+    RETURN (m < n div 8 \<or> n-m < n div 8)
+  }"
 
+  lemma bad_partition_triv: "m\<le>n \<Longrightarrow> bad_partition m n \<le> SPEC (\<lambda>_. True)"
+    unfolding bad_partition_def
+    apply refine_vcg
+    by simp
+  
+  abbreviation "par_sort_seq_threshold::nat \<equiv> 100000"  
+  abbreviation "ppar_chunk_size::nat \<equiv> 1000000"  
     
-    lemma par_sort_aux2_refine: "n=length xs \<Longrightarrow> par_sort_aux2 xs n d \<le> \<Down>(\<langle>Id\<rangle>list_rel) (par_sort_aux xs d)"
-      unfolding par_sort_aux2_def par_sort_aux_def nres_par_def
-      apply (refine_rcg)
-      supply [refine_dref_RELATES] = RELATESI[where R="{((xs,n,d),(xs',d')). xs'=xs \<and> d'=d \<and> length xs'=n}"]
-      apply refine_dref_type
-      apply (simp_all (no_asm_use)) (* TODO: This is a hack against a yet unidentified simplifier loop *)
-      apply auto
-      done
+  definition "par_sort_aux xs d \<equiv> RECT (\<lambda>par_sort_aux (xs,d::nat). doN {
+    let n = length xs;
+    if d=0 \<or> n<par_sort_seq_threshold then
+      slice_sort_spec (\<^bold><) xs 0 n
+    else doN {
+      (xs',m) \<leftarrow> partition3_spec xs 0 n;
+      bad \<leftarrow> bad_partition m n;
+      
+      ASSERT (length xs' = length xs);
+      (_,xs'') \<leftarrow> WITH_SPLIT m xs' (\<lambda>xs\<^sub>1 xs\<^sub>2. doN {
+        ASSERT (length xs' = length xs\<^sub>1 + length xs\<^sub>2);
+        (xs\<^sub>1',xs\<^sub>2') \<leftarrow> if bad then doN {
+          xs\<^sub>1' \<leftarrow> par_sort_aux (xs\<^sub>1,d-1);
+          ASSERT (length xs\<^sub>1' = length xs\<^sub>1);
+          xs\<^sub>2' \<leftarrow> par_sort_aux (xs\<^sub>2,d-1);
+          ASSERT (length xs\<^sub>2' = length xs\<^sub>2);
+          RETURN (xs\<^sub>1',xs\<^sub>2')
+        } else doN {
+          xs\<^sub>1' \<leftarrow> par_sort_aux (xs\<^sub>1,d-1);
+          ASSERT (length xs\<^sub>1' = length xs\<^sub>1);
+          xs\<^sub>2' \<leftarrow> par_sort_aux (xs\<^sub>2,d-1);
+          ASSERT (length xs\<^sub>2' = length xs\<^sub>2);
+          RETURN (xs\<^sub>1',xs\<^sub>2')
+        };
+        RETURN ((),xs\<^sub>1',xs\<^sub>2')
+      });
+      RETURN xs''
+    }
+  }) (xs,d)"
+  
+  
+  lemma par_sort_aux_correct: "par_sort_aux xs d \<le> slice_sort_spec (\<^bold><) xs 0 (length xs)"
+    unfolding par_sort_aux_def 
+    apply (subst if_cancel)
+    apply (refine_vcg RECT_rule_arb[where V="measure (\<lambda>(_,d). d)" and pre="\<lambda>xss (xs,d). xss=xs"])
+    apply simp_all [2]
+    unfolding slice_sort_spec_def partition3_spec_def
+    apply (refine_vcg bad_partition_triv)
+    apply simp_all 
+    apply (meson slice_eq_mset_all slice_eq_mset_def)
+    apply (rule order_trans) apply (rprems)
+    apply simp
+    apply simp
+    apply refine_vcg
+    apply (clarsimp)
+    apply (rule order_trans) apply (rprems)
+    apply simp
+    apply simp
+    apply refine_vcg
+    apply (clarsimp_all)
+    subgoal for xs' xs\<^sub>2' xs\<^sub>1 xs\<^sub>2 xc x1b
+      
+      unfolding sort_spec_def slice_eq_mset_def slice_LT_def
+      apply (auto simp: slice_complete' sorted_wrt_append le_by_lt slice_append1' slice_append2')
+      by (metis set_mset_mset)
+    done
+    
+  text \<open>Introducing explicit parameter for list length\<close>  
+  definition "par_sort_aux2 xs n d \<equiv> RECT (\<lambda>par_sort_aux (xs,n,d::nat). doN {
+    ASSERT (n = length xs);
+    if d=0 \<or> n<par_sort_seq_threshold then
+      slice_sort_spec (\<^bold><) xs 0 n
+    else doN {
+      (xs,m) \<leftarrow> partition3_spec xs 0 n;
+      bad \<leftarrow> bad_partition m n;
+      (_,xs) \<leftarrow> WITH_SPLIT m xs (\<lambda>xs\<^sub>1 xs\<^sub>2. doN {
+        ASSERT (length xs\<^sub>2 = length xs - m);
+        ASSERT (n\<ge>m);
+        (xs\<^sub>1,xs\<^sub>2) \<leftarrow> if bad then doN {
+          xs\<^sub>1 \<leftarrow> par_sort_aux (xs\<^sub>1,m,d-1);
+          xs\<^sub>2 \<leftarrow> par_sort_aux (xs\<^sub>2,n-m,d-1);
+          RETURN (xs\<^sub>1,xs\<^sub>2)
+        } else doN {
+          nres_par par_sort_aux par_sort_aux (xs\<^sub>1,m,d-1) (xs\<^sub>2,n-m,d-1)
+        };
+        RETURN ((),xs\<^sub>1,xs\<^sub>2)
+      });
+      RETURN xs
+    }
+  }) (xs,n,d)"
+
+  
+  lemma par_sort_aux2_refine: "n=length xs \<Longrightarrow> par_sort_aux2 xs n d \<le> \<Down>(\<langle>Id\<rangle>list_rel) (par_sort_aux xs d)"
+    unfolding par_sort_aux2_def par_sort_aux_def nres_par_def
+    apply (refine_rcg)
+    supply [refine_dref_RELATES] = RELATESI[where R="{((xs,n,d),(xs',d')). xs'=xs \<and> d'=d \<and> length xs'=n}"]
+    apply refine_dref_type
+    apply (simp_all (no_asm_use)) (* TODO: This is a hack against a yet unidentified simplifier loop *)
+    apply auto
+    done
 
 
 
   text \<open>Fixing concrete algorithms to be used\<close>
+  
+  text \<open>Version with sequential partitioner\<close>
   definition "par_sort_aux3 xs n d \<equiv> RECT (\<lambda>par_sort_aux (xs,n,d::nat). doN {
     ASSERT (n = length xs);
     if d=0 \<or> n<par_sort_seq_threshold then
@@ -145,6 +147,7 @@ context weak_ordering begin
   }) (xs,n,d)"
 
   
+  text \<open>Version with parallel partitioner\<close>
   definition "ppar_sort_aux3 xs n d \<equiv> RECT (\<lambda>par_sort_aux (xs,n,d::nat). doN {
     ASSERT (n = length xs);
     if d=0 \<or> n<par_sort_seq_threshold then
@@ -424,14 +427,5 @@ context sort_impl_copy_context begin
     
 
 end
-
-
-
-
-
-
-
-
-
 
 end
